## C++

### Dynamic Programming
Define P(i,j) as following:

P(i,j) = { true,  if the substring Si … Sj is a palindrome <br>
           false, otherwise. <br>
}

Therefore,

P(i, j) = (P(i+1, j−1) and Si == Sj)

1. allocate a 2D array, and fill `1` for all (i, i) (i from 0 to n-1)
2. For every length (from 1 to n-1): <br>
     For every position (from 0 to n-1): <br>
        check palindrome for each segment. This can reuse the work of i-1 for length i. <br>

```C++
class Solution {
public:
    string longestPalindrome(string s) {
        vector<vector<int>> v(s.size(), vector<int>(s.size(), 0));
        for(int i = 0; i < s.size(); i++) {
            v[i][i] = 1;
        }
        
        int r1 = 0, r2 = 0, r_len = 1;
        for(int j = 1; j < s.size(); j++) {
            for(int i = 0; i < s.size(); i++) {            
                if (i + j >= s.size()) continue;
                int a = i, b = i + j;
                if (s[a] != s[b]) continue;
                
                if (b - a <= 2 || v[a+1][b-1] > 0) {
                    if (b - a <= 2) {
                        v[a][b] = b - a + 1;
                    } else {
                        v[a][b] = v[a+1][b-1] + 2;
                    }
                    if (v[a][b] > r_len) {
                        r_len = v[a][b];
                        r1 = a, r2 = b;
                    }
                }
            }
        }
        return s.substr(r1, r2 - r1 + 1);
    }
};
```

### Expand around centers
```C++
class Solution {
private:
    int findStr(const string& s, int& a, int& b) {
        while(a >= 0 && b < s.size() && s[a] == s[b]) {
            a--, b++;
        }
        a++, b--;
        if (a > b) return 0;
        return b-a+1;
    }
public:
    string longestPalindrome(string s) {
        int s0 = 0, e0 = 0;
        for(int i = 1; i < s.size(); i++) {
            int a = i-1, b = i+1;
            int r = findStr(s, a, b);
            if (r > (e0-s0+1)) {
                s0 = a;
                e0 = b;
            }
            a = i-1;
            b = i;
            r = findStr(s, a, b);
            if (r > (e0-s0+1)) {
                s0 = a;
                e0 = b;
            }
        }
        return s.substr(s0, e0-s0+1);
    }
};
```
