# 0779. K-th Symbol in Grammar, medium, , freq: 2.%, acceptance: 37.6%

On the first row, we write a 0. Now in every subsequent row, we look at the previous row and replace each occurrence of 0 with 01, and each occurrence of 1 with 10.

Given row N and index K, return the K-th indexed symbol in row N. (The values of K are 1-indexed.) (1 indexed).

Examples:
Input: N = 1, K = 1
Output: 0

Input: N = 2, K = 1
Output: 0

Input: N = 2, K = 2
Output: 1

Input: N = 4, K = 5
Output: 1

Explanation:
row 1: 0
row 2: 01
row 3: 0110
row 4: 01101001
Note:

N will be an integer in the range [1, 30].
K will be an integer in the range [1, 2^(N-1)].

```c++
// 0ms, 100%
class Solution {
public:
    int kthGrammar(int N, int K) {
        /*
        0
        01
        0110
        0110 1001
        0110 1001 1001 0110
        0110 1001 1001 0110 1001 0110 0110 1001
        */
        if (N == 1) return 0;

        // K starts from 1
        // if parent is 0, pos (K%2 == 1) is 0, pos (K%2 == 0) is 1
        // if parent is 1, pos (K%2 == 1) is 1, pos (K%2 == 0) is 0
        return (1-K%2) ^ kthGrammar(N-1, (K+1)/2);
    }
};

// 4ms, 53%
class Solution {
public:
    int kthGrammar(int N, int K) {
        /*
        0
        01
        0110
        0110 1001
        0110 1001 1001 0110
        0110 1001 1001 0110 1001 0110 0110 1001
        */
        if (N == 1) return 0;
        // second half is flip of the first half
        // so if K is in second half, flip
        if (K <= (1 << (N-2)))
            return kthGrammar(N-1, K);
        return 1 ^ kthGrammar(N-1, K - (1 << (N-2)));
    }
};

// MLE
class Solution {
public:
    int kthGrammar(int N, int K) {
        /*
        0
        01
        0110
        0110 1001
        0110 1001 1001 0110
        0110 1001 1001 0110 1001 0110 0110 1001
        */
        string s = "0110";
        while (s.size() < K) {
            int sz = s.size();
            auto half = sz/2;
            s += s.substr(half) + s.substr(0, half);
        }
        return s[K-1] - '0';
    }
};
```
